checkpoint

src/Spec/Example.v
@@ -1,6 +1,8 @@
 Require Import Helpers.Helpers.
 Require Import Helpers.ListStuff.
 Require Import ConcurProc.
+Require Import Equiv.
+Require Import Omega.
 
 Global Set Implicit Arguments.
 Global Generalizable All Variables.
@@ -119,3 +121,118 @@ Proof.
 Defined.
 
 Eval compute in (proj1_sig ex_trace2).
+
+
+Theorem ex_trace_ex_trace2 :
+  traces_match (proj1_sig ex_trace) (proj1_sig ex_trace2).
+Proof.
+  simpl.
+  eauto 20.
+Qed.
+
+
+(** Compilation *)
+
+Inductive compile_ok : forall `(p1 : proc opT opHiT T) `(p2 : proc opHiT opHi2T T), Prop :=
+| CompileIncTwice :
+  compile_ok (inc_twice_impl) (Op IncTwice)
+| CompileRet : forall `(x : T),
+  compile_ok (Ret x) (Ret x)
+| CompileBind : forall `(p1a : proc opT opHiT T1) (p2a : proc opHiT opHi2T T1)
+                       `(p1b : T1 -> proc opT opHiT T2) (p2b : T1 -> proc opHiT opHi2T T2),
+  compile_ok p1a p2a ->
+  (forall x, compile_ok (p1b x) (p2b x)) ->
+  compile_ok (Bind p1a p1b) (Bind p2a p2b).
+
+Hint Constructors compile_ok.
+
+Theorem ex_compile_ok : compile_ok p1 p2.
+Proof.
+  unfold p1, p2.
+  eauto.
+Qed.
+
+Hint Resolve ex_compile_ok.
+
+
+Definition threads_compile_ok (ts1 : @threads_state opT opHiT) (ts2 : @threads_state opHiT opHi2T) :=
+  forall tid,
+    ts1 [[ tid ]] = NoProc /\ ts2 [[ tid ]] = NoProc \/
+  (exists T (p1 : proc _ _ T) p2,
+    ts1 [[ tid ]] = Proc p1 /\ ts2 [[ tid ]] = Proc p2 /\ compile_ok p1 p2).
+
+Theorem ex_ts_compile_ok : threads_compile_ok ts ts2.
+Proof.
+  unfold threads_compile_ok, ts, ts2, thread_upd, threads_empty; intros.
+  destruct tid; subst; compute; eauto.
+  destruct tid; subst; compute; eauto 10.
+  destruct tid; subst; compute; eauto.
+Qed.
+
+
+Ltac thread_inv :=
+  match goal with
+  | H : thread_get (thread_upd _ _ _) _ = Proc _ |- _ =>
+    eapply thread_upd_inv in H; destruct H; (intuition idtac); subst
+  | H : thread_get threads_empty _ = Proc _ |- _ =>
+    eapply thread_empty_inv in H; exfalso; apply H
+  | H : (_, _) = (_, _) |- _ =>
+    inversion H; clear H; subst; repeat sigT_eq
+  | H : _ = Bind _ _ |- _ =>
+    solve [ inversion H ]
+  | H : _ = Ret _ |- _ =>
+    solve [ inversion H ]
+  | H : no_runnable_threads (thread_upd _ _ _) |- _ =>
+    solve [ eapply thread_upd_not_empty in H; exfalso; eauto ]
+  | H : _ _ = Proc _ |- _ =>
+    solve [ exfalso; eapply no_runnable_threads_some; eauto ]
+  | H : _ = _ |- _ =>
+    congruence
+  | H : _ = _ \/ _ = _ |- _ =>
+    solve [ intuition congruence ]
+  | H : ?a = ?a |- _ =>
+    clear H
+  end || maybe_proc_inv.
+
+Ltac bind_inv :=
+  match goal with
+  | H : _ = Bind _ _ |- _ =>
+    inversion H; clear H; subst; repeat sigT_eq
+  end.
+
+Ltac exec_inv :=
+  match goal with
+  | H : exec _ _ _ _ |- _ =>
+    inversion H; clear H; subst
+  end;
+  autorewrite with t in *.
+
+Ltac empty_inv :=
+  try solve [ exfalso; eapply thread_empty_inv; eauto ].
+
+Ltac step_inv :=
+  match goal with
+  | H : op_step _ _ _ _ _ |- _ =>
+    inversion H; clear H; subst; repeat sigT_eq
+  | H : opHi_step _ _ _ _ _ |- _ =>
+    inversion H; clear H; subst; repeat sigT_eq
+  end.
+
+
+Theorem ex_all_traces_match :
+  forall s tr1 tr2,
+  exec op_step s ts tr1 ->
+  exec opHi_step s ts2 tr2 ->
+  traces_match tr1 tr2.
+Proof.
+  intros.
+  unfold ts, ts2 in *.
+
+  repeat ( exec_inv; repeat thread_inv;
+    try ( repeat exec_tid_inv; repeat thread_inv ) ).
+  repeat step_inv.
+
+  unfold inc, state_upd; simpl.
+  replace (s' 1 + 1 + 1) with (s' 1 + 2) by omega.
+  eauto 20.
+Qed.
